specs/Spec.HMAC_DRBG.Vectors.fst
@@ -74,6 +74,9 @@ type vec = {
   nonce: hex_string;
   personalization_string: hex_string;
   entropy_input_reseed: hex_string;
+  additional_input_reseed: hex_string;
+  additional_input_1: hex_string;
+  additional_input_2: hex_string;  
   returned_bits: hex_string;
 }
 
@@ -84,7 +87,21 @@ let test_vectors : list vec = [
   nonce = "1146733abf8c35c8";
   personalization_string = "";
   entropy_input_reseed = "c7215b5b96c48e9b338c74e3e99dfedf";
+  additional_input_reseed = "";
+  additional_input_1 = "";
+  additional_input_2 = "";
   returned_bits = "c6a16ab8d420706f0f34ab7fec5adca9d8ca3a133e159ca6ac43c6f8a2be22834a4c0a0affb10d7194f1c1a5cf7322ec1ae0964ed4bf122746e087fdb5b3e91b3493d5bb98faed49e85f130fc8a459b7";
+  };
+  {
+  a = SHA1;
+  entropy_input = "c2e9a6e2e29f47dee0e808660c446a4f";
+  nonce = "aff465073a97862c";
+  personalization_string = "";
+  entropy_input_reseed = "2ab6787095e944c5276d29bbbbd7a777";
+  additional_input_reseed = "358ffeab6a24f932abd4c9577f84cb13";
+  additional_input_1 = "37578c2d9b68d43d6c83164a4c43ce37";
+  additional_input_2 = "02a7c9575d9527a33df9fb566373db3a";
+  returned_bits = "fcd318c83563f72e5a21d4a93a84254e0c3bb6d3ded55c3d5939dbd5d1525062fd587a422012437aeb88589e669e5a5d57f7ebb16e30590f6debd0eced84f8e57d47a3d123a52361145a8fab258ed19b";
   };
   {
   a = SHA2_256;
@@ -92,7 +109,21 @@ let test_vectors : list vec = [
   nonce = "0e66f71edc43e42a45ad3c6fc6cdc4df";
   personalization_string = "";
   entropy_input_reseed = "01920a4e669ed3a85ae8a33b35a74ad7fb2a6bb4cf395ce00334a9c9a5a5d552";  
+  additional_input_reseed = "";
+  additional_input_1 = "";
+  additional_input_2 = "";
   returned_bits = "76fc79fe9b50beccc991a11b5635783a83536add03c157fb30645e611c2898bb2b1bc215000209208cd506cb28da2a51bdb03826aaf2bd2335d576d519160842e7158ad0949d1a9ec3e66ea1b1a064b005de914eac2e9d4f2d72a8616a80225422918250ff66a41bd2f864a6a38cc5b6499dc43f7f2bd09e1e0f8f5885935124";
+  };
+  {
+  a = SHA2_256;
+  entropy_input = "93161b2dc08cb0fd50171141c865a841ca935cfdd2b5907d6ff8ab0348c4ceb0";
+  nonce = "5cb9f6e5912b90c3349a50ab881b35a1";
+personalization_string =  "0dceb4a36326c4df1685df43fddeecb5d0c76f00eb44826694f27e610290f6e1";
+  entropy_input_reseed = "d8e9be44b5f293482548d4787762ebfb03c73c40e45385e8b98907cd66f493dd";
+  additional_input_reseed = "105a8f85d6959f3e043ef508cfea21d52123f03b7aea8034c4eec761eaba1fee";
+  additional_input_1 = "bf781f7e489d9b4b5aa5ee6d1796468af672a8d25f311edf3c4b4dbf433d703f";
+  additional_input_2 = "c81d6bcf1e5bf37e39dda1735c6f193df115b1a854a12e7cafe060afe4589335";
+  returned_bits = "4306628124d0100fade7eaaf5edf227d50771f9e5f2e1e983800eef9a39fde0b0c280e63c8728d836b5b93ea794a32c1c04cfc54bd5300e3febb5fe2e1023eded8d7cd180279a598f76823e8d5a7dffcc93a09deec5d1f80838e938fba4de9f47e94b99382ae55f116df9c3b3ddf7e50516e203645852a415796f03a86418107";
   };
   {
   a = SHA2_384;
@@ -100,6 +131,9 @@ let test_vectors : list vec = [
   nonce = "fc7983b918acadaa71a67e1624f1b502";
   personalization_string = "";
   entropy_input_reseed = "4260a0495fdaba58aae41df82505012d480c8e4f751fd7ebc39f9becd694b2a3";
+  additional_input_reseed = "";
+  additional_input_1 = "";
+  additional_input_2 = "";
   returned_bits = "f4c7bec0c26cf3892d214549ac6f3d82f34c6966d4295099ee56166e879a70ecae130251facda351e903d877b6c5eab5153ce87ba6c7cf8bcc61cbd14cfbe34cf1ed43678aee69cd87b60e6bcb6ff48ebd44ce9e31982d8fe20aec34fa51d625f845f61056575969bf785c2ffab4dcc754f13de63423e94bad8d5e166d96a62a602d3ee4045df162028b89cac45e6207d9097f2b3ac0ab17729251985f276f1287f5c56cc9ba1a79fbdbb291f3a945fbfdbd63cf13b82ec91f7b1085b33279e3";
   };
   {
@@ -108,6 +142,9 @@ let test_vectors : list vec = [
   nonce = "bbb7c777428068fad9970891f879b1af";
   personalization_string = "";  
   entropy_input_reseed = "e0ffefdadb9ccf990504d568bdb4d862cbe17ccce6e22dfcab8b4804fd21421a";
+  additional_input_reseed = "";
+  additional_input_1 = "";
+  additional_input_2 = "";
   returned_bits = "05da6aac7d980da038f65f392841476d37fe70fbd3e369d1f80196e66e54b8fadb1d60e1a0f3d4dc173769d75fc3410549d7a843270a54a068b4fe767d7d9a59604510a875ad1e9731c8afd0fd50b825e2c50d062576175106a9981be37e02ec7c5cd0a69aa0ca65bddaee1b0de532e10cfa1f5bf6a026e47379736a099d6750ab121dbe3622b841baf8bdcbe875c85ba4b586b8b5b57b0fecbec08c12ff2a9453c47c6e32a52103d972c62ab9affb8e728a31fcefbbccc556c0f0a35f4b10ace2d96b906e36cbb72233201e536d3e13b045187b417d2449cad1edd192e061f12d22147b0a176ea8d9c4c35404395b6502ef333a813b6586037479e0fa3c6a23";
   };
 ]
