specs/Spec.HMAC_DRBG.fst
@@ -21,6 +21,7 @@ let reseed_interval   = pow2 48
 let max_output_length = pow2 16
 let max_length        = pow2 16
 let max_personalization_string_length = pow2 16
+let max_additional_input_length = pow2 16
 
 /// See p.54
 /// https://nvlpubs.nist.gov/nistpubs/SpecialPublications/NIST.SP.800-57pt1r4.pdf
@@ -38,38 +39,39 @@ type state (a:supported_alg) =
   -> state a
 
 val hmac_input_bound: a:supported_alg -> Lemma 
-  (hash_length a + pow2 32 + 1 + block_length a + block_length a <= max_input_length a)
+  (hash_length a + pow2 32 + pow2 32 + 1 + block_length a + block_length a <= max_input_length a)
 let hmac_input_bound = function
   | SHA1     -> 
     let a = SHA1 in
-    assert_norm (hash_length a + pow2 32 + 1 + block_length a + block_length a <= max_input_length a)
+    assert_norm (hash_length a + pow2 32 + pow2 32 +1 + block_length a + block_length a <= max_input_length a)
   | SHA2_256 ->   
     let a = SHA2_256 in
-    assert_norm (hash_length a + pow2 32 + 1 + block_length a + block_length a <= max_input_length a)
+    assert_norm (hash_length a + pow2 32 + pow2 32 + 1 + block_length a + block_length a <= max_input_length a)
   | SHA2_384 -> 
     let a = SHA2_384 in
-    assert_norm (hash_length a + pow2 32 + 1 + block_length a + block_length a <= max_input_length a)
+    assert_norm (hash_length a + pow2 32 + pow2 32 + 1 + block_length a + block_length a <= max_input_length a)
   | SHA2_512 -> 
     let a = SHA2_512 in
-    assert_norm (hash_length a + pow2 32 + 1 + block_length a + block_length a <= max_input_length a)
+    assert_norm (hash_length a + pow2 32 + pow2 32 + 1 + block_length a + block_length a <= max_input_length a)
 
 val update: #a:supported_alg
   -> data:bytes
-  -> state a 
-  -> Pure (state a)
+  -> k:lbytes (hash_length a)
+  -> v:lbytes (hash_length a)
+  -> Pure (lbytes (hash_length a) & lbytes (hash_length a))
   (requires hash_length a + Seq.length data + 1 + block_length a <= max_input_length a)
   (ensures  fun _ -> True)
-let update #a data (State k v ctr) =
+let update #a data k v =
   let zero_data = Seq.cons (u8 0) data in
   let k = hmac a k (v @| zero_data) in
   let v = hmac a k v in
   if Seq.length data = 0 then
-    State k v ctr
+    k, v
   else
     let one_data = Seq.cons (u8 1) data in
     let k = hmac a k (v @| one_data) in
     let v = hmac a k v in
-    State k v ctr
+    k, v 
 
 (* We omit personalization_string *)
 val instantiate: #a:supported_alg
@@ -88,17 +90,23 @@ let instantiate #a entropy_input nonce personalization_string =
   let seed_material = entropy_input @| nonce @| personalization_string in
   let k = Seq.create (hash_length a) (u8 0) in
   let v = Seq.create (hash_length a) (u8 1) in  
-  update #a seed_material (State k v 1)
+  let k, v = update #a seed_material k v in
+  State k v 1
 
 val reseed: #a:supported_alg
   -> state a
   -> entropy_input: bytes
+  -> additional_input: bytes
   -> Pure (state a)
   (requires 
-    hash_length a + Seq.length entropy_input + 1 + block_length a <= max_input_length a)
+    hash_length a + 
+    Seq.length entropy_input + 
+    Seq.length additional_input +
+    1 + block_length a <= max_input_length a)
   (ensures fun _ -> True)
-let reseed #a st entropy_input =
-  let State k v _ = update #a entropy_input st in
+let reseed #a st entropy_input additional_input =
+  let seed_material = entropy_input @| additional_input in
+  let k, v = update #a seed_material st.k st.v in
   State k v 1
 
 let a_spec (a:hash_alg) (i:nat) = Lib.Sequence.lseq uint8 (hash_length a)
@@ -120,12 +128,20 @@ let generate_loop a k max i vi =
 val generate: #a:supported_alg
   -> state a
   -> n:pos{n <= max_output_length}
-  -> option (lbytes n & state a)
-let generate #a (State k v ctr) n =
+  -> additional_input: bytes
+  -> Pure (option (lbytes n & state a))
+  (requires hash_length a + Seq.length additional_input + 1 + block_length a <= max_input_length a)
+  (ensures fun _ -> True)
+let generate #a st n additional_input =
   hmac_input_bound a;
-  if ctr > reseed_interval then 
+  if st.reseed_counter > reseed_interval then 
     None
-  else    
+  else
+    let k, v = 
+      if Seq.length additional_input > 0 then
+        update additional_input st.k st.v 
+      else st.k, st.v
+    in
     let max = n / hash_length a in
     let v, output =
       Lib.Sequence.generate_blocks (hash_length a) max max (a_spec a)
@@ -139,19 +155,27 @@ let generate #a (State k v ctr) n =
       else
         v, output
     in
-    let State k v _ = update Seq.empty (State k v ctr) in
-    Some (output, State k v (ctr + 1))
+    let k, v = update additional_input k v in
+    Some (output, State k v (st.reseed_counter + 1))
 
 (** Equivalently, but proving it requires proving extensionality of generate_blocks *)
 val generate': #a:supported_alg
   -> state a
   -> n:pos{n <= max_output_length}
-  -> option (lbytes n & state a)
-let generate' #a (State k v ctr) n =
+  -> additional_input: bytes
+  -> Pure (option (lbytes n & state a))
+  (requires hash_length a + Seq.length additional_input + 1 + block_length a <= max_input_length a)
+  (ensures fun _ -> True)
+let generate' #a st n additional_input =
   hmac_input_bound a;
-  if ctr > reseed_interval then 
+  if st.reseed_counter > reseed_interval then 
     None
   else    
+    let k, v = 
+      if Seq.length additional_input > 0 then
+        update additional_input st.k st.v 
+      else st.k, st.v
+    in
     // let max = ceil (n / hash_length a) in
     let max = (n + hash_length a - 1) / hash_length a in
     let v, output =
@@ -159,5 +183,5 @@ let generate' #a (State k v ctr) n =
         (generate_loop a k max)
         v
     in
-    let State k v _ = update Seq.empty (State k v ctr) in
-    Some (Seq.slice output 0 n, State k v (ctr + 1))
+    let k, v = update additional_input k v in
+    Some (Seq.slice output 0 n, State k v (st.reseed_counter + 1))
